examples/elliptic/arm/mlton/bsubstML.sml
@@ -1,12 +1,28 @@
 structure bsubstML :> bsubstML =
 struct
-  nonfix empty_memory MEM_ITEMS MEM_WRITE_BLOCK MEM_WRITE MEM_WRITE_WORD
-         MEM_WRITE_BYTE MEM_READ SET_BYTE ADDR30 ::- :- * / div mod + -
-         ^ @ <> > < >= <= := o before;
+  nonfix MEM_WRITE MEM_WRITE_WORD MEM_WRITE_HALF MEM_WRITE_BYTE SET_HALF
+         SET_BYTE FORMAT GET_BYTE GET_HALF ADDR30 mem_items empty_memory
+         mem_write_block mem_write mem_read ::- :- data_size Word Half
+         Byte formats_size UnsignedWord UnsignedHalfWord SignedHalfWord
+         UnsignedByte SignedByte * / div mod + - ^ @ <> > < >= <= := o
+         before;
   
   open numML fcpML wordsML;
   type mem = (word30, word32) Redblackmap.dict
   val mem_updates = ref ([]: word30 list)
+  datatype formats
+       = SignedByte
+       | UnsignedByte
+       | SignedHalfWord
+       | UnsignedHalfWord
+       | UnsignedWord
+  fun formats_size x = ZERO
+    
+  datatype data = Byte of word8 | Half of word16 | Word of word32
+  fun data_size (Byte(a)) = ONE
+    | data_size (Half(a)) = ONE
+    | data_size (Word(a)) = ONE
+    
   fun :- a b = fn m => fn c => if a = c then b else m c
     
   fun ::- a l =
@@ -14,8 +30,76 @@ struct
         if word_ls a b andalso < (- (w2n b) (w2n a)) (listML.LENGTH l)
           then listML.EL (- (w2n b) (w2n a)) l else m b
     
+  fun fromHexNum s n =
+        wordsML.fromNum(numML.fromHexString n, fcpML.Tyop (s, []));
+
+  val fromNum32 = (fromHexNum "i32"): string -> word32;
+
+  fun mem_read (m,a) = Redblackmap.find(m:mem, a)
+                       handle NotFound => fromNum32 "E6000010";
+    
+  fun mem_write m a d = (:= (mem_updates, a :: !mem_updates);
+                         Redblackmap.insert(m:mem, a, d));
+    
+  fun mem_write_block m a [] = m
+    | mem_write_block m a (d::l) =
+        mem_write_block (mem_write m a d)
+          (word_add a (n2w_itself (ONE,(Tyop ("i30", []))))) l
+    
+  fun word_compare(v, w) =
+    let val m = w2n v and n = w2n w in
+      if m = n then
+        EQUAL
+      else
+        if < m n then LESS else GREATER
+    end
+
+  val empty_memory = (Redblackmap.mkDict word_compare):mem
+
+  fun mem_items m = Redblackmap.listItems m
+    
   fun ADDR30 addr =
         word_extract_itself (Tyop ("i30", [])) (fromString"31") TWO addr
+    
+  fun GET_HALF oareg data =
+        if index oareg ONE
+          then word_extract_itself (Tyop ("i16", [])) (fromString"31")
+                 (fromString"16") data
+          else word_extract_itself (Tyop ("i16", [])) (fromString"15")
+                 ZERO data
+    
+  fun GET_BYTE oareg data =
+        case word_eq oareg (n2w_itself (ZERO,(Tyop ("i2", []))))
+         of true =>
+               word_extract_itself (Tyop ("i8", [])) (fromString"7")
+                 ZERO data
+          | false =>
+               (case word_eq oareg (n2w_itself (ONE,(Tyop ("i2", []))))
+                of true =>
+                      word_extract_itself (Tyop ("i8", []))
+                        (fromString"15") (fromString"8") data
+                 | false =>
+                      (case
+                         word_eq oareg
+                           (n2w_itself (TWO,(Tyop ("i2", []))))
+                       of true =>
+                             word_extract_itself (Tyop ("i8", []))
+                               (fromString"23") (fromString"16") data
+                        | false =>
+                             word_extract_itself (Tyop ("i8", []))
+                               (fromString"31") (fromString"24") data))
+    
+  fun FORMAT fmt oareg data =
+        case fmt
+         of SignedByte =>
+               sw2sw_itself (Tyop ("i32", [])) (GET_BYTE oareg data)
+          | UnsignedByte =>
+               w2w_itself (Tyop ("i32", [])) (GET_BYTE oareg data)
+          | SignedHalfWord =>
+               sw2sw_itself (Tyop ("i32", [])) (GET_HALF oareg data)
+          | UnsignedHalfWord =>
+               w2w_itself (Tyop ("i32", [])) (GET_HALF oareg data)
+          | UnsignedWord => data
     
   fun SET_BYTE oareg b w =
         word_modify (fn i => fn x =>
@@ -40,46 +124,38 @@ struct
                   (n2w_itself ((fromString"3"),(Tyop ("i2", []))))
                then index b (- i (fromString"24")) else x)))) w
     
-  fun fromHexNum s n =
-        wordsML.fromNum(numML.fromHexString n, fcpML.Tyop (s, []));
-
-  val fromNum32 = (fromHexNum "i32"): string -> word32;
-
-  fun MEM_READ(m,a) = Redblackmap.find(m, a)
-                       handle NotFound => fromNum32 "E6000010";
+  fun SET_HALF oareg hw w =
+        word_modify (fn i => fn x =>
+          < i (fromString"16")
+          andalso
+          (if not oareg then index hw i else x)
+          orelse
+          (<= (fromString"16") i andalso < i (fromString"32"))
+          andalso
+          (if oareg then index hw (- i (fromString"16")) else x)) w
     
   fun MEM_WRITE_BYTE mem addr word =
         let val addr30 = ADDR30 addr
         in
-           Redblackmap.insert(mem, (addr30: word30),
-             SET_BYTE
+           mem_write mem addr30
+             (SET_BYTE
                 (word_extract_itself (Tyop ("i2", [])) ONE ZERO addr)
-                (word_extract_itself (Tyop ("i8", [])) (fromString"7")
-                   ZERO word) (MEM_READ(mem,addr30)))
+                word (mem_read (mem,addr30)))
         end
-
-  fun MEM_WRITE_WORD (mem:mem) addr word =
-        Redblackmap.insert(mem,ADDR30 addr,word)
-
-  fun MEM_WRITE b m a =
-        (:= (mem_updates, ADDR30 a :: !mem_updates);
-          if b then MEM_WRITE_BYTE m a else MEM_WRITE_WORD m a)
-
-  fun MEM_WRITE_BLOCK m (a: word30) [] = m
-    | MEM_WRITE_BLOCK m a (d::l) =
-       (:= (mem_updates, ADDR30 a :: !mem_updates);
-        MEM_WRITE_BLOCK (Redblackmap.insert(m, a, (d: word32)))
-          (word_add a (n2w_itself (ONE,(Tyop ("i30", []))))) l)
     
-  fun MEM_ITEMS (m:mem) = Redblackmap.listItems m
-
-  fun word_compare(v, w) =
-    let val m = w2n v and n = w2n w in
-      if m = n then
-        EQUAL
-      else
-        if < m n then LESS else GREATER
-    end
-
-  val empty_memory = (Redblackmap.mkDict word_compare):mem
+  fun MEM_WRITE_HALF mem addr word =
+        let val addr30 = ADDR30 addr
+        in
+           mem_write mem addr30
+             (SET_HALF (index addr ONE) word (mem_read (mem,addr30)))
+        end
+    
+  fun MEM_WRITE_WORD mem addr word = mem_write mem (ADDR30 addr) word
+    
+  fun MEM_WRITE mem addr d =
+        case d
+         of Byte(b) => MEM_WRITE_BYTE mem addr b
+          | Half(hw) => MEM_WRITE_HALF mem addr hw
+          | Word(w) => MEM_WRITE_WORD mem addr w
+    
 end
